vacid/union_find.ml
@@ -1,20 +1,18 @@
 (** Union find represented using pointers *)
 
-type cell = { 
-  mutable parent : content;
-  mutable rank : int }
+type cell = content ref
 and content = Node of cell | Root
 
 let rec repr x =
-   match x.parent with
+   match !x with
    | Root -> x
    | Node y -> 
-      let r = repr y in
-      x.parent <- Node r;
-      r
+       let r = repr y in
+       x := Node r;
+       r
 
 let create () = 
-   { parent = Root; rank = 0 }
+   ref Root
 
 let same x y =
   repr x == repr y
@@ -22,13 +20,7 @@ let same x y =
 let union x y =
    let rx = repr x in
    let ry = repr y in
-   if rx != ry then begin
-      if rx.rank < ry.rank then
-         rx.parent <- Node ry
-      else if rx.rank > ry.rank then
-         ry.parent <- Node rx
-      else (
-         ry.parent <- Node rx;
-         rx.rank <- ry.rank + 1)
-   end 
+   if rx != ry 
+      then rx := Node ry 
+
 
